Update subtyping

Coq/Coq34.v
@@ -164,3 +164,352 @@ Module Examples2.
 
 End Examples2.
 
+Lemma sub_inversion_Bool : ∀U,
+     U <: Bool' →
+     U = Bool'.
+Proof with auto.
+  intros U Hs.
+  remember Bool' as V.
+  induction Hs;inversion HeqV;auto.
+  apply IHHs2 in H;subst. auto.
+Qed.
+
+Lemma sub_inversion_arrow : ∀U V1 V2,
+     U <: Arrow' V1 V2 →
+     ∃U1 U2,
+     U = Arrow' U1 U2 ∧ V1 <: U1 ∧ U2 <: V2.
+Proof with eauto.
+  intros U V1 V2 Hs.
+  remember (Arrow' V1 V2) as V.
+  generalize dependent V2. generalize dependent V1.
+  induction Hs;intros.
+  3 : inversion HeqV.
+  - exists V1, V2;auto.
+  - apply IHHs2 in HeqV;inversion HeqV;inversion H;clear HeqV H.
+    destruct H0. apply IHHs1 in H;inversion H;inversion H1;clear H H1.
+    exists x1, x2. inversion H2. inversion H1. clear H2 H1.
+    split;destruct H0...
+  - inversion HeqV;subst. exists S1, S2...
+Qed.
+
+Require Import Coq.Program.Equality.
+
+Lemma canonical_forms_of_arrow_types : ∀Gamma s T1 T2,
+  Gamma ⊢ s ∈ Arrow' T1 T2 →
+  value' s →
+  ∃x S1 s2,
+     s = abs' x S1 s2.
+Proof with eauto.
+  intros Gamma s T1 T2 H. dependent induction H;intros H';subst...
+  1 - 3 : inversion H'.
+  apply sub_inversion_arrow in H0. destruct H0 as [U1 (U2, (H1, (H2, H3)))].
+  apply IHhas_type' in H1...
+Qed.
+
+Ltac solve_by_inverts n :=
+  match goal with | H : ?T |- _ =>
+  match type of T with Prop =>
+    solve [
+      inversion H;
+      match n with S (S (?n')) => subst; solve_by_inverts (S n') end ]
+  end end.
+
+Ltac solve_by_invert := solve_by_inverts 1.
+
+Lemma canonical_forms_of_Bool : ∀Gamma s,
+  Gamma ⊢ s ∈ Bool' →
+  value' s →
+  s = tru' ∨ s = fls'.
+Proof with eauto.
+  intros Gamma s Hty Hv.
+  remember Bool' as T.
+  induction Hty; try solve_by_invert...
+  subst;apply sub_inversion_Bool in H;subst...
+Qed.
+
+Theorem progress' : ∀t T,
+     empty ⊢ t ∈ T →
+     value' t ∨ ∃t', t ---> t'.
+Proof with eauto.
+  intros t T Ht.
+  remember empty as Gamma.
+  revert HeqGamma.
+  induction Ht;
+    intros HeqGamma; subst...
+  -  inversion H.
+  - right.
+    destruct IHHt1; subst...
+    + destruct IHHt2; subst...
+      * destruct (canonical_forms_of_arrow_types empty t1 T1 T2)
+          as [x [S1 [t12 Heqt1]]]...
+        subst. exists ([x:=t2]t12)...
+      * inversion H0 as [t2' Hstp]. exists (app' t1 t2')...
+    + inversion H as [t1' Hstp]. exists (app' t1' t2)...
+  - right.
+    destruct IHHt1.
+    + eauto.
+    + assert (t1 = tru' ∨ t1 = fls')
+        by (eapply canonical_forms_of_Bool; eauto).
+      inversion H0; subst...
+    + inversion H. rename x into t1'. eauto.
+Qed.
+
+Lemma typing_inversion_abs : ∀Gamma x S1 t2 T,
+     Gamma ⊢ (abs' x S1 t2) ∈ T →
+     ∃S2,
+       Arrow' S1 S2 <: T
+       ∧ (x ⊢> S1 ; Gamma) ⊢ t2 ∈ S2.
+Proof with eauto.
+  intros Gamma x S1 t2 T H.
+  remember (abs' x S1 t2) as t.
+  induction H;
+    inversion Heqt; subst; intros; try solve_by_invert.
+  - (* T_Abs *)
+    exists T12...
+  - (* T_Sub *)
+    destruct IHhas_type' as [S2 [Hsub Hty]]...
+  Qed.
+
+Lemma typing_inversion_var : ∀Gamma x T,
+  Gamma ⊢ (var' x) ∈ T →
+  exists S,
+    Gamma x = Some S ∧ S <: T.
+Proof with eauto.
+  intros Gamma x T Hty.
+  remember (var' x) as t.
+  induction Hty; intros;
+    inversion Heqt; subst; try solve_by_invert.
+  - (* T_Var *)
+    exists T...
+  - (* T_Sub *)
+    destruct IHHty as [U [Hctx HsubU]]... Qed.
+
+Lemma typing_inversion_app : ∀Gamma t1 t2 T2,
+  Gamma ⊢ (app' t1 t2) ∈ T2 →
+  exists T1,
+    Gamma ⊢ t1 ∈ (Arrow' T1 T2) ∧
+    Gamma ⊢ t2 ∈ T1.
+Proof with eauto.
+  intros Gamma t1 t2 T2 Hty.
+  remember (app' t1 t2) as t.
+  induction Hty; intros;
+    inversion Heqt; subst; try solve_by_invert.
+  - (* T_App *)
+    exists T1...
+  - (* T_Sub *)
+    destruct IHHty as [U1 [Hty1 Hty2]]...
+Qed.
+
+Lemma typing_inversion_true : ∀Gamma T,
+  Gamma ⊢ tru' ∈ T →
+  Bool' <: T.
+Proof with eauto.
+  intros Gamma T Htyp. remember tru' as tu.
+  induction Htyp;
+    inversion Heqtu; subst; intros...
+Qed.
+
+Lemma typing_inversion_false : ∀Gamma T,
+  Gamma ⊢ fls' ∈ T →
+  Bool' <: T.
+Proof with eauto.
+  intros Gamma T Htyp. remember fls' as tu.
+  induction Htyp;
+    inversion Heqtu; subst; intros...
+Qed.
+
+Lemma typing_inversion_if : ∀Gamma t1 t2 t3 T,
+  Gamma ⊢ (test' t1 t2 t3) ∈ T →
+  Gamma ⊢ t1 ∈ Bool'
+  ∧ Gamma ⊢ t2 ∈ T
+  ∧ Gamma ⊢ t3 ∈ T.
+Proof with eauto.
+  intros Gamma t1 t2 t3 T Hty.
+  remember (test' t1 t2 t3) as t.
+  induction Hty; intros;
+    inversion Heqt; subst; try solve_by_invert.
+  - (* T_Test *)
+    auto.
+  - (* T_Sub *)
+    destruct (IHHty H0) as [H1 [H2 H3]]...
+Qed.
+
+Lemma typing_inversion_unit : ∀Gamma T,
+  Gamma ⊢ unit ∈ T →
+    Unit <: T.
+Proof with eauto.
+  intros Gamma T Htyp. remember unit as tu.
+  induction Htyp;
+    inversion Heqtu; subst; intros...
+Qed.
+
+Lemma abs_arrow : ∀x S1 s2 T1 T2,
+  empty ⊢ (abs' x S1 s2) ∈ (Arrow' T1 T2) →
+     T1 <: S1
+  ∧ (x ⊢> S1 ; empty) ⊢ s2 ∈ T2.
+Proof with eauto.
+  intros x S1 s2 T1 T2 Hty.
+  apply typing_inversion_abs in Hty.
+  inversion Hty as [S2 [Hsub Hty1]].
+  apply sub_inversion_arrow in Hsub.
+  inversion Hsub as [U1 [U2 [Heq [Hsub1 Hsub2]]]].
+  inversion Heq; subst... Qed.
+
+Inductive appears_free_in : string → tms → Prop :=
+  | afi_var : ∀x,
+      appears_free_in x (var' x)
+  | afi_app1 : ∀x t1 t2,
+      appears_free_in x t1 → appears_free_in x (app' t1 t2)
+  | afi_app2 : ∀x t1 t2,
+      appears_free_in x t2 → appears_free_in x (app' t1 t2)
+  | afi_abs : ∀x y T11 t12,
+        y ≠ x →
+        appears_free_in x t12 →
+        appears_free_in x (abs' y T11 t12)
+  | afi_test1 : ∀x t1 t2 t3,
+      appears_free_in x t1 →
+      appears_free_in x (test' t1 t2 t3)
+  | afi_test2 : ∀x t1 t2 t3,
+      appears_free_in x t2 →
+      appears_free_in x (test' t1 t2 t3)
+  | afi_test3 : ∀x t1 t2 t3,
+      appears_free_in x t3 →
+      appears_free_in x (test' t1 t2 t3)
+.
+
+Hint Constructors appears_free_in.
+
+Theorem beq_string_refl : ∀ s, true = beq_string s s. 
+Proof. 
+  intros s. unfold beq_string. destruct (string_dec s s) as [|Hs]. 
+  - reflexivity.   
+  - destruct Hs. reflexivity. 
+Qed.
+
+Theorem beq_string_false_iff : ∀ x y : string,   beq_string x y = false ↔ x ≠ y. 
+Proof. 
+  intros x y. rewrite <- beq_string_true_iff. 
+  rewrite not_true_iff_false. reflexivity. 
+Qed.
+
+Theorem false_beq_string : ∀ x y : string, x ≠ y → beq_string x y = false. 
+Proof. 
+  intros x y. rewrite beq_string_false_iff. 
+  intros H. apply H. 
+Qed.
+
+Lemma context_invariance : ∀Gamma Gamma' t S,
+     Gamma ⊢ t ∈ S →
+     (∀x, appears_free_in x t → Gamma x = Gamma' x) →
+     Gamma' ⊢ t ∈ S.
+Proof with eauto.
+  intros. generalize dependent Gamma'.
+  induction H;
+    intros Gamma' Heqv...
+  - (* T_Var *)
+    apply T_Var... rewrite <- Heqv...
+  - (* T_Abs *)
+    apply T_Abs... apply IHhas_type'. intros x0 Hafi.
+    unfold update, t_update. destruct (eqb_spec x x0)...
+    subst. rewrite <- beq_string_refl...
+    specialize (false_beq_string _ _ n);intros;rewrite H0...
+  - (* T_Test *)
+    apply T_Test'...
+Qed.
+
+Lemma free_in_context : ∀x t T Gamma,
+   appears_free_in x t →
+   Gamma ⊢ t ∈ T →
+   ∃T', Gamma x = Some T'.
+Proof with eauto.
+  intros x t T Gamma Hafi Htyp.
+  induction Htyp;
+      subst; inversion Hafi; subst...
+  - (* T_Abs *)
+    destruct (IHHtyp H4) as [T Hctx]. exists T.
+    unfold update, t_update in Hctx.
+    rewrite <- beq_string_false_iff in H2.
+    rewrite H2 in Hctx... Qed.
+
+Lemma substitution_preserves_typing : ∀Gamma x U v t S,
+     (x ⊢> U ; Gamma) ⊢ t ∈ S →
+     empty ⊢ v ∈ U →
+     Gamma ⊢ [x:=v]t ∈ S.
+Proof with eauto.
+  intros Gamma x U v t S Htypt Htypv.
+  generalize dependent S. generalize dependent Gamma.
+  induction t; intros; simpl.
+  - (* var *)
+    rename s into y.
+    destruct (typing_inversion_var _ _ _ Htypt)
+        as [T [Hctx Hsub]].
+    unfold update, t_update in Hctx.
+    destruct (eqb_spec x y) as [Hxy|Hxy]; eauto;
+    subst. rewrite <- beq_string_refl in *.
+    inversion Hctx; subst. clear Hctx.
+    apply context_invariance with empty...
+    intros x Hcontra.
+    destruct (free_in_context _ _ S empty Hcontra)
+        as [T' HT']...
+    inversion HT'.
+    specialize (false_beq_string _ _ Hxy);intros;rewrite H in *...
+  - (* app *)
+    destruct (typing_inversion_app _ _ _ _ Htypt)
+        as [T1 [Htypt1 Htypt2]].
+    eapply T_App...
+  - (* abs *)
+    rename s into y. rename t into T1.
+    destruct (typing_inversion_abs _ _ _ _ _ Htypt)
+      as [T2 [Hsub Htypt2]].
+    apply T_Sub with (Arrow' T1 T2)... apply T_Abs...
+    destruct (eqb_spec x y) as [Hxy|Hxy].
+    + (* x=y *)
+      eapply context_invariance...
+      subst.
+      intros x Hafi. unfold update, t_update.
+      destruct (eqb_spec y x);subst. rewrite <- beq_string_refl in *...
+      specialize (false_beq_string _ _ n);intros;rewrite H in *...
+    + (* x<>y *)
+      apply IHt. eapply context_invariance...
+      intros z Hafi. unfold update, t_update.
+      destruct (eqb_spec y z)...
+      subst. rewrite <- beq_string_refl...
+      specialize (false_beq_string _ _ Hxy);intros;rewrite H in *...
+      rewrite <- beq_string_false_iff in Hxy.
+      specialize (false_beq_string _ _ n);intros;rewrite H in *...
+  - (* tru *)
+      assert (Bool' <: S)
+        by apply (typing_inversion_true _ _ Htypt)...
+  - (* fls *)
+      assert (Bool' <: S)
+        by apply (typing_inversion_false _ _ Htypt)...
+  - (* test *)
+    assert ((x ⊢> U ; Gamma) ⊢ t1 ∈ Bool'
+         ∧ (x ⊢> U ; Gamma) ⊢ t2 ∈ S
+         ∧ (x ⊢> U ; Gamma) ⊢ t3 ∈ S)
+      by apply (typing_inversion_if _ _ _ _ _ Htypt).
+    inversion H as [H1 [H2 H3]].
+    apply IHt1 in H1. apply IHt2 in H2. apply IHt3 in H3.
+    auto.
+  - (* unit *)
+    assert (Unit <: S)
+      by apply (typing_inversion_unit _ _ Htypt)...
+Qed.
+
+Theorem preservation' : ∀t t' T,
+     empty ⊢ t ∈ T →
+     t ---> t' →
+     empty ⊢ t' ∈ T.
+Proof with eauto.
+  intros t t' T HT.
+  remember empty as Gamma. generalize dependent HeqGamma.
+  generalize dependent t'.
+  induction HT;
+    intros t' HeqGamma HE; subst; inversion HE; subst...
+  - (* T_App *)
+    inversion HE; subst...
+    + (* ST_AppAbs *)
+      destruct (abs_arrow _ _ _ _ _ HT1) as [HA1 HA2].
+      apply substitution_preserves_typing with T...
+Qed.
+
